code cleanup after merge

execution/tests/CongressGens.v
@@ -1,7 +1,7 @@
 From ConCert Require Import Blockchain LocalBlockchain Congress.
 From ConCert Require Import Serializable.
 From ConCert Require Import BoundedN ChainedList.
-From ConCert.Execution.QCTests Require Import ChainGens TestUtils ChainPrinters CongressPrinters SerializablePrinters.
+From ConCert.Execution.QCTests Require Import TestUtils ChainPrinters CongressPrinters SerializablePrinters.
 
 Require Import ZArith Strings.Ascii Strings.String.
 
@@ -25,7 +25,7 @@ Notation "f 'o' g" := (compose f g) (at level 50).
 
 (* ChainGens for the types defined in the Congress contract *)
 
-Definition LocalChainBase : ChainBase := ChainGens.LocalChainBase.
+Definition LocalChainBase : ChainBase := TestUtils.LocalChainBase.
 
 Definition gRulesSized (n : nat) : G Rules :=
   vote_count <- choose(1%Z, 1000%Z) ;;
@@ -41,198 +41,7 @@ Instance genSetupSized : GenSized Setup :=
 {|
   arbitrarySized n := liftM build_setup (arbitrarySized n)
 |}.
-
-Definition gCongressAction' {ctx : ChainContext LocalChainBase}
-                           (gMsg : G SerializedValue) 
-                           : G CongressAction :=
-  freq [
-    (1, liftM2 cact_transfer (ctx_gAccountAddr ctx) gZPositive);
-    (1, liftM3 cact_call (ctx_gContractAddr ctx) gZPositive gMsg)
-  ].
-
-Definition gMsgSimple (ctx : ChainContext LocalChainBase) : G Msg := 
-  freq [
-    (1, liftM transfer_ownership (ctx_gAccountAddr ctx)) ;
-    (1, liftM change_rules arbitrary) ;
-    (2, liftM add_member (ctx_gAccountAddr ctx)) ;
-    (2, liftM remove_member (ctx_gAccountAddr ctx)) ;
-    (2, liftM vote_for_proposal arbitrary) ;
-    (2, liftM vote_against_proposal arbitrary) ;
-    (2, liftM retract_vote arbitrary) ;
-    (2, liftM finish_proposal arbitrary)
-  ].
-Definition gMsg' : G Msg := 
-  ctx <- arbitrary ;; gMsgSimple ctx.
-
-(* Sample gMsg'.
-Sample (ctx <- @arbitrarySized _ genLocalChainContext 1 ;; @gCongressAction' ctx (liftM serializeMsg (gMsgSimple ctx))).
-
-Sample (ctx <- @arbitrarySized _ genLocalChainContext 1 ;; 
-        ctx_gAccountAddr ctx). *)
-
-Fixpoint gMsgSized (ctx : ChainContext LocalChainBase) (n : nat) : G Msg :=
-  let default := liftM add_member (ctx_gAccountAddr ctx) in
-  match n with
-    | 0 => gMsgSimple ctx
-    | S n' => freq [
-        (1,
-        (* recurse. Msg is converted to a SerializedType using 'serialize' *)
-        (* This makes it possible to create proposals about proposals about proposals etc... *)
-        congressActions <- listOf (@gCongressAction' ctx (liftM serializeMsg (gMsgSized ctx n'))) ;;
-        returnGen (create_proposal congressActions)) ;
-        (7, gMsgSimple ctx)
-      ]
-  end.
-
-(* Sample (ctx <- arbitrary ;; @gMsgSized ctx 1). *)
-
-Example ex_simple_msg : Msg := create_proposal [cact_transfer zero_address 1%Z ].
-Example ex_msg : Msg := create_proposal [cact_call zero_address 0%Z (serialize Msg _ ex_simple_msg)].
-Compute ((show o (deserialize Msg _) o serializeMsg) ex_simple_msg).
-Compute (show ex_msg). 
-
-(* Generates semantically valid/well-formed messages *)
-(* Examples of validity requirements: 
-   - retract_vote can only be called on a proposal if it there exists a vote on this proposal 
-*)
-Definition gValidSimpleMsg (ctx : ChainContext LocalChainBase) 
-                           (proposals : FMap nat Proposal) 
-                           : G Msg  := 
-  let proposals_pairlist := FMap.elements proposals in
-  let proposalIds := map fst proposals_pairlist in
-  let proposalIds_and_votes := map (fun p => (fst p, votes (snd p))) proposals_pairlist in
-  let proposalIds_with_votes : list nat := fold_left (fun acc p => if FMap.size (snd p) =? 0 then acc else (fst p) :: acc) proposalIds_and_votes [] in 
-  let retract_vote_weight := if length proposalIds_with_votes  =? 0 then 0 else 2 in
-  let vote_proposal_weight := if length proposalIds =? 0 then 0 else 2 in
-  default_pid <- arbitrary ;;
-  freq [
-    (1, liftM transfer_ownership (ctx_gAccountAddr ctx)) ;
-    (1, liftM change_rules arbitrary) ;
-    (2, liftM add_member (ctx_gAccountAddr ctx)) ;
-    (2, liftM remove_member (ctx_gAccountAddr ctx)) ;
-    (vote_proposal_weight, liftM vote_for_proposal (elems_ default_pid proposalIds)) ;
-    (vote_proposal_weight, liftM vote_against_proposal (elems_ default_pid proposalIds)) ;
-    (vote_proposal_weight, liftM finish_proposal (elems_ default_pid proposalIds)) ;
-    (retract_vote_weight, 
-      pid <- elems_ default_pid proposalIds_with_votes ;;
-      returnGen (retract_vote pid))
-  ].
-
-Definition gCongressActionSized {ctx : ChainContext LocalChainBase}
-                                (n : nat)
-                                : G CongressAction 
-                                := @gCongressAction' ctx (liftM serializeMsg (@gMsgSized ctx n)).
-
-(* Sample (ctx <- arbitrary ;; gMsgSized ctx 2). *)
-
-Example ex_call_congress_action := ctx <- arbitrary ;; 
-                                   liftM (cact_call zero_address 0%Z) (liftM serializeMsg (gMsgSized ctx 2) ).
-(* Sample ex_call_congress_action. *)
-
-Open Scope Z_scope.
-
-Definition gProposalSized {ctx : ChainContext LocalChainBase} 
-                          (proposed_in : nat) (* obtained from the Chain *)
-                          (nr_votes : nat)
-                          (n : nat)
-                                   : G Proposal :=
-  bound <- arbitrarySized n ;;
-  actions <- vectorOf bound (@gCongressActionSized ctx n) ;;
-  vote_vals <- vectorOf nr_votes (elems [-1%Z; 1%Z]) ;; (* -1 = vote against, 1 = vote for*) 
-  votes <- gFMapFromInput (ctx_accounts ctx) vote_vals ;;
-  let vote_result := fold_left Z.add (FMap.values votes) 0%Z in
-  (* vote_result <- choose (-(Z.of_nat nr_votes), Z.of_nat nr_votes);; *)
-  returnGen (build_proposal actions votes vote_result proposed_in).
-
-(* Sample (ctx <- arbitrary ;; @gProposalSized ctx 0 10 1). *)
-
-Close Scope Z_scope.
-
-Definition gStateSized {ctx : ChainContext LocalChainBase} 
-                       (current_slot : nat) (* used to ensure that the generated proposals are never proposed at a later date *)
-                       (n : nat) 
-                       : G Congress.State :=
-  let nr_accounts := length (ctx_accounts ctx) in
-  default_addr <- (ctx_gAccountAddr ctx) ;;
-  owner <- elems_ default_addr (ctx_accounts ctx) ;; (* owner is a member *)
-  rules <- arbitrarySized n ;;
-  proposalIds <- vectorOfCount 0 n ;;
-  nr_votes <- choose (1, if nr_accounts =? 0 then 1 else nr_accounts) ;;
-  proposals <- vectorOf n (slot <- (arbitrarySized current_slot) ;; @gProposalSized ctx slot nr_votes  (n/2)) ;;
-  proposals_map <- gFMapFromInput proposalIds proposals ;;
-  next_proposal_id <- arbitrary ;; (* TODO: maybe just let it be 0*)
-  unit_list <- (vectorOf nr_accounts (returnGen tt)) ;;
-  members <- gFMapFromInput (ctx_accounts ctx) unit_list ;;
-  returnGen (build_state owner rules proposals_map next_proposal_id members).
-
-Definition gProposalIdFromState (state : Congress.State) : G ProposalId := 
-  let pelems := FMap.elements (proposals state) in
-  let pids := map fst pelems in
-  (* Choose one proposal id at random. If empty, choose an arbitrary one. *)
-  default_pid <- arbitrary ;; elems_ default_pid  pids.
-
-Definition gProposalFromState {ctx : ChainContext LocalChainBase} 
-                              (state : Congress.State)
-                              (proposed_in : nat) 
-                              : G Proposal := 
-  let pelems := FMap.elements (proposals state) in
-  let pids := map snd pelems in
-  let max_nr_votes : nat := (length o FMap.elements) (members state) in
-  (* Choose one proposal id at random. If empty, choose an arbitrary one. *)
-  nr_votes <- arbitrarySized max_nr_votes ;;
-  default_proposal <- @gProposalSized ctx proposed_in nr_votes 3 ;; 
-  elems_ default_proposal pids.
-
-Definition gCongressContract : G (Contract Setup Msg Congress.State) :=
-  returnGen Congress.contract.
   
-(* Sample gCongressContract. *)
-
-Definition gValidContractCallContext {ctx : ChainContext LocalChainBase}
-                                            (owner_addr : Address) 
-                                            (msg : Msg)
-                                            : G (@ContractCallContext LocalChainBase) := 
-  match msg with
-  (* these messages must be created by the owner of the congress *)
-  | change_rules _ | add_member _ | remove_member _ | transfer_ownership _ => gContractCallContextWithOwner ctx owner_addr 
-  | _ => gContractCallContext ctx 
-  end.
-  
-(* Sample (ctx <-arbitrarySized 4 ;; state <- @gStateSized ctx 10 2 ;; msg <- gMsgSized ctx 3 ;; @gValidContractCallContextFromMsg ctx state msg). *)
-
-Definition receive_is_some_P chain ctx state msg := 
-  match (receive chain ctx state (Some msg)) with
-  | Some _ => true
-  | None => false
-  end.
-  
-Definition check_receive_is_some_P := 
-  forAll5
-    (gLocalChainContext 4)
-    (fun ctx => gLocalChainSized 2 ctx)
-    (fun ctx chain => @gStateSized ctx (current_slot chain) 2)
-    (fun ctx cctx state => gValidSimpleMsg ctx (proposals state))
-    (fun ctx _ state msg => @gValidContractCallContext ctx (owner state) msg)
-    (fun _ chain state msg cctx => receive_is_some_P chain cctx state msg).
-
-(* We expect to get fail this test at this point*)
-(* QuickChick check_receive_is_some_P. *)
-(* coqtop-stdout:ChainContext{...}
-Chain{height: 2, current slot: 0, final height: 1}
-State{owner: 7%256, rules: Rules{min_vote_count_permille: 2, margin_needed_permille: 2, debating_period_in_blocks: 4}, proposals: ["0-->Proposal{actions: [(transfer: 121%256, 4)], votes: [\"121%256-->-1\"], vote_result: 1, proposed_in: 0, }\n"; "1-->Proposal{actions: [(call: 179%256, 1, SerializedValue{(4,(((1,(161,(4,((8,(5,())),())))),((0,(111,(4,()))),((0,(8,(4,()))),()))),()))})], votes: [\"121%256-->-1\"], vote_result: 4, proposed_in: 0, }\n"], next_proposal_id: 5, members: ["7%256-->tt"; "121%256-->tt"; "125%256-->tt"; "110%256-->tt"]}
-(finish_proposal 1)
-ContractCallContext{ctx_from: 121%256, ctx_contract_addr: 143%256, ctx_amount: 5}
-*** Failed after 13 tests and 0 shrinks. (0 discards) 
-*)
-
-Definition gActionOfCongress ctx n : G Action := 
-  liftM2 (@build_act LocalChainBase) (ctx_gAccountAddr ctx) (liftM congress_action_to_chain_action (@gCongressActionSized ctx n)).
-
-Definition gContractCallInfo := liftM3 build_call_info arbitrary arbitrary arbitrary.
-  
-(* Sample gContractCallInfo. *)
-
-(* ------------------------------------------------------ *)
 (* generators of actions from the LocalChain context type *)
 
 Definition allProposalsOfLC lc : FMap ProposalId Proposal := 
