execution/tests/EIP20TokenPrinters.v
@@ -1,6 +1,6 @@
 From ConCert Require Import Blockchain LocalBlockchain.
 From ConCert Require Import EIP20Token.
-From ConCert.Execution.QCTests Require Import ChainGens TestUtils ChainPrinters.
+From ConCert.Execution.QCTests Require Import TestUtils ChainPrinters.
 Require Import Strings.String.
 From QuickChick Require Import QuickChick.
 
